unusedVar.v
@@ -47,3 +47,29 @@ sigT (fun T:Type => sig (fun (f:T) =>
 forall po, 
 let V_R : BestRel V V₂ := {| R:= Rp; Rtot := pt ; Rone := po|} in
 JMeq (P V V₂ V_R) f)).
+
+Definition existsAGoodnessFreeImpl2 
+{T: forall (A A₂ : Set) (A_R : BestRel A A₂) (B B₂ : Set) (B_R : BestRel B B₂), Type}
+(P : forall (A A₂ : Set) (A_R : BestRel A A₂)
+(B B₂ : Set) (B_R : BestRel B B₂) , T A A₂ A_R B B₂ B_R) : Type :=
+forall 
+(A A₂ : Set) (Ra: (A -> A₂ -> Prop))
+(B B₂ : Set) (Rb: (B -> B₂ -> Prop)),
+sigT (fun T:Type => sig (fun (f:T) =>
+forall pta poa ptb pob, 
+let A_R : BestRel A A₂ := {| R:= Ra; Rtot := pta ; Rone := poa|} in
+let B_R : BestRel B B₂ := {| R:= Rb; Rtot := ptb ; Rone := pob|} in
+JMeq (P A A₂ A_R B B₂ B_R) f)).
+
+Definition existsAOneFreeImpl2 
+{T: forall (A A₂ : Set) (A_R : BestRel A A₂) (B B₂ : Set) (B_R : BestRel B B₂), Type}
+(P : forall (A A₂ : Set) (A_R : BestRel A A₂)
+(B B₂ : Set) (B_R : BestRel B B₂) , T A A₂ A_R B B₂ B_R) : Type :=
+forall 
+(A A₂ : Set) (Ra: (A -> A₂ -> Prop)) pta 
+(B B₂ : Set) (Rb: (B -> B₂ -> Prop)) ptb,
+sigT (fun T:Type => sig (fun (f:T) =>
+forall poa pob, 
+let A_R : BestRel A A₂ := {| R:= Ra; Rtot := pta ; Rone := poa|} in
+let B_R : BestRel B B₂ := {| R:= Rb; Rtot := ptb ; Rone := pob|} in
+JMeq (P A A₂ A_R B B₂ B_R) f)).
