test-suite/iso/squiggle5.v
@@ -1,0 +1,164 @@
+Require Import ReflParam.common.
+Require Import ReflParam.templateCoqMisc.
+Require Import String.
+Require Import List.
+Require Import Template.Ast.
+Require Import SquiggleEq.terms.
+Require Import ReflParam.paramDirect ReflParam.indType.
+Require Import ReflParam.indProp.
+Require Import SquiggleEq.substitution.
+Require Import ReflParam.PiTypeR.
+Import ListNotations.
+Open Scope string_scope.
+
+Require Import ReflParam.Trecord.
+
+
+Set Imlicit Arguments.
+
+Inductive eqs {A : Set} (x : A) : forall (a:A), Prop :=  
+  eq_refls : eqs x x.
+
+Inductive option (A : Set) : Set :=  Some : A -> option A | None : option A.
+Arguments Some {A} _.
+Arguments None {A}.
+
+Infix "=" := eqs : type_scope.
+Notation True := (true=true).
+Notation False := (false=true).
+
+Definition isNone {A:Set} (oa: option A) :=
+  match oa with
+  | Some _ => false
+  | None => true
+  end.
+Infix "+" := sum:type_scope.
+(*
+Definition beq (b1 b2 : bool) := eqs bool b1 b2.
+ *)
+
+
+Open Scope nat_scope.
+
+Section Squiggle5.
+  (* Variable V:Set. This interface is too abstract for exposing V *)
+Variables (Tm BTm : Set).
+Variable applyBtm: BTm -> Tm -> Tm.
+
+Inductive TmKind :=
+| elam (bt: BTm) 
+| eapp (f a: Tm) 
+| enum (n: nat)
+| evar.
+
+Variable tmKind:  Tm -> TmKind.
+
+Fixpoint evaln (n:nat) (t:Tm): option Tm :=
+match n with
+| 0 => None | S n => 
+  match (tmKind t)
+  with
+  | evar => None
+  | elam _ | enum _ => Some t
+  | eapp f a =>
+    match evaln n f, evaln n a with
+    | Some f, Some a =>
+      match (tmKind f) with
+      | elam bt => evaln n (applyBtm bt a)
+      | _ => None
+      end
+    | _,_ => None
+    end
+  end
+end.
+
+
+(* just this would be an example. However, because it is not recursive,
+ even tauto may be able to prove it. Even if we only show this on paper,
+we should have a more complex (recursively defined undefined relation)
+in the appendix *)
+Definition divergesIff (tl tr:Tm) : Prop :=
+  (forall (nsteps:nat), (isNone (evaln nsteps tl)) = true) <->
+  (forall (nsteps:nat), (isNone (evaln nsteps tr)) = true).
+
+ (* need to eliminate the oneOne of Prop inductives and use PI *)
+ 
+(*  
+(fun _ => 0) 2
+(fun _ => 0) 4
+
+This rule will judge the above to be different. We never see inside non-canonical
+terms!
+ | eapp fl al , eapp fr ar => obsEq k fl fr /\ obsEq k al ar 
+*)
+
+Fixpoint obsEq (k:nat) (tl tr:Tm) {struct k}: Prop :=
+divergesIff tl tr /\ forall (nsteps:nat), 
+match k with | 0 => True | S k =>
+  match evaln nsteps tl, evaln nsteps tr with
+  | Some vl, Some vr => 
+     match tmKind vl, tmKind vr with
+     | enum nl , enum nr => nl = nr
+     | elam btl , elam btr => forall (ta: Tm), obsEq k (applyBtm btl ta) (applyBtm btr ta)
+     | _,_ => False
+     end
+  | _, _  => True
+  end
+end.
+
+
+End Squiggle5.
+
+Arguments elam {Tm} {BTm} bt.
+Arguments eapp {Tm} {BTm} f a.
+Arguments enum {Tm} {BTm} n.
+Arguments evar {Tm} {BTm}.
+
+
+Run TemplateProgram (genParamIndAll [] "Coq.Init.Datatypes.bool").
+Run TemplateProgram (genParamIndAll [] "Coq.Init.Datatypes.nat").
+Run TemplateProgram (genParamIndPropAll [] "Top.squiggle5.eqs").
+Run TemplateProgram (genParamIndAll [] "Top.squiggle5.option").
+
+(* and, unlike exists, allows singleton elim because the 2 args of its constructor
+are proofs *)
+Run TemplateProgram (genParamIndPropAll [] "Coq.Init.Logic.and").
+Run TemplateProgram (genParamIndAll [] "Top.squiggle5.TmKind").
+
+Run TemplateProgram (mkIndEnv "indTransEnv" [
+"Coq.Init.Datatypes.bool" ; "Coq.Init.Datatypes.nat";
+(* "Coq.Init.Logic.and";  "Top.squiggle5.eqs"; *)
+ "Top.squiggle5.option"; 
+ (* "Top.squiggle2.sum";  "Top.squiggle2.list"; "Top.squiggle2.prod"; *)
+ "Top.squiggle5.TmKind"]).
+
+Run TemplateProgram (genWrappers indTransEnv).
+
+Run TemplateProgram (genParam indTransEnv true true "Top.squiggle5.evaln").
+(* slow and the result is bloated *)
+
+Run TemplateProgram (genParam indTransEnv true true "Top.squiggle5.isNone").
+
+Run TemplateProgram (genParam indTransEnv true true "Coq.Init.Logic.iff").
+
+
+Run TemplateProgram (genParam indTransEnv true true "Top.squiggle5.divergesIff").
+(* quick *)
+Run TemplateProgram (genParam indTransEnv true true "Top.squiggle5.obsEq").
+(* bloated *)
+
+Require Import ReflParam.unusedVar.
+
+(*
+Lemma obsEqExistsAOneFreeImpl  : existsAOneFreeImpl2
+  (Top_squiggle5_obsEq_pmtcty_RR).
+Proof.
+  eexists.
+  eexists.
+  intros.
+  set (fvv:= Top_squiggle5_obsEq_pmtcty_RR _ _ A_R _ _ B_R).
+  simpl in *.
+  lazy in fvv.
+  reflexivity.
+Defined.
+*)
